prove trace-based property of counter

systems/Counter.v
@@ -144,7 +144,7 @@ Section Counter.
     break_match; find_inversion; auto.
   Qed.
 
-  Definition in_flight (l : list packet) : nat :=
+  Definition inc_in_flight_to_backup (l : list packet) : nat :=
     length (filterMap
               (fun p => if msg_eq_dec (pBody p) inc
                      then if name_eq_dec (pDst p) backup
@@ -152,38 +152,38 @@ Section Counter.
                      else None)
               l).
 
-  Lemma in_flight_app :
+  Lemma inc_in_flight_to_backup_app :
     forall xs ys,
-      in_flight (xs ++ ys) = in_flight xs + in_flight ys.
+      inc_in_flight_to_backup (xs ++ ys) = inc_in_flight_to_backup xs + inc_in_flight_to_backup ys.
   Proof.
     intros.
-    unfold in_flight.
+    unfold inc_in_flight_to_backup.
     rewrite filterMap_app.
     rewrite app_length.
     auto.
   Qed.
 
-  Lemma in_flight_cons_primary_dst :
+  Lemma inc_in_flight_to_backup_cons_primary_dst :
     forall p,
       pDst p = primary ->
-      in_flight [p] = 0.
+      inc_in_flight_to_backup [p] = 0.
   Proof.
     intros.
-    unfold in_flight.
+    unfold inc_in_flight_to_backup.
     simpl.
     repeat break_match; try congruence; auto.
   Qed.
 
-  Lemma in_flight_nil :
-    in_flight [] = 0.
+  Lemma inc_in_flight_to_backup_nil :
+    inc_in_flight_to_backup [] = 0.
   Proof.
     reflexivity.
   Qed.
 
-  Lemma InputHandler_in_flight_preserved :
+  Lemma InputHandler_inc_in_flight_to_backup_preserved :
     forall h i d u o d' l,
       InputHandler h i d = (u, o, d', l) ->
-      d' = d + in_flight (send_packets h l).
+      d' = d + inc_in_flight_to_backup (send_packets h l).
   Proof.
     unfold InputHandler, PrimaryInputHandler, BackupInputHandler.
     simpl.
@@ -193,16 +193,16 @@ Section Counter.
     rewrite plus_comm. auto.
   Qed.
 
-  Lemma NetHandler_in_flight_preserved :
+  Lemma NetHandler_inc_in_flight_to_backup_preserved :
     forall p d u o d' l,
       NetHandler (pDst p) (pBody p) d = (u, o, d', l) ->
-      d' + in_flight (send_packets (pDst p) l) = d + in_flight [p].
+      d' + inc_in_flight_to_backup (send_packets (pDst p) l) = d + inc_in_flight_to_backup [p].
   Proof.
     unfold NetHandler, PrimaryNetHandler, BackupNetHandler.
     intros.
     monad_unfold.
     destruct p. simpl in *.
-    repeat break_match; find_inversion; simpl; try rewrite in_flight_nil;
+    repeat break_match; find_inversion; simpl; try rewrite inc_in_flight_to_backup_nil;
     unfold Data in *; compute;
     auto with *.
   Qed.
@@ -229,7 +229,7 @@ Section Counter.
   Lemma backup_plus_network_eq_primary :
     forall net tr,
       step_m_star (params := Counter_MultiParams) step_m_init net tr ->
-      nwState net backup + in_flight (nwPackets net) = nwState net primary.
+      nwState net backup + inc_in_flight_to_backup (nwPackets net) = nwState net primary.
   Proof.
     intros.
     remember step_m_init as y in *.
@@ -241,28 +241,28 @@ Section Counter.
       | [ H : step_m _ _ _ |- _ ] => invc H
       end; simpl.
       + find_apply_lem_hyp net_handlers_NetHandler.
-        find_copy_apply_lem_hyp NetHandler_in_flight_preserved.
+        find_copy_apply_lem_hyp NetHandler_inc_in_flight_to_backup_preserved.
         repeat find_rewrite.
         rewrite cons_is_app in IHrefl_trans_1n_trace1.
-        repeat rewrite in_flight_app in *.
+        repeat rewrite inc_in_flight_to_backup_app in *.
         destruct (pDst p) eqn:?;
                  try rewrite update_same;
           try rewrite update_diff by congruence;
           unfold send_packets in *; simpl in *.
         * erewrite PrimaryNetHandler_no_msgs with (ms := l) in * by eauto.
-          rewrite in_flight_cons_primary_dst in * by auto.
-          simpl in *. rewrite in_flight_nil in *. auto with *.
+          rewrite inc_in_flight_to_backup_cons_primary_dst in * by auto.
+          simpl in *. rewrite inc_in_flight_to_backup_nil in *. auto with *.
         * omega.
       + find_apply_lem_hyp input_handlers_InputHandlers.
-        find_copy_apply_lem_hyp InputHandler_in_flight_preserved.
+        find_copy_apply_lem_hyp InputHandler_inc_in_flight_to_backup_preserved.
         unfold send_packets in *. simpl in *.
-        rewrite in_flight_app. subst.
+        rewrite inc_in_flight_to_backup_app. subst.
         destruct h eqn:?;
                  try rewrite update_same;
           try rewrite update_diff by congruence.
         * omega.
         * erewrite InputHandler_backup_no_msgs with (l := l) by eauto.
-          simpl. rewrite in_flight_nil. omega.
+          simpl. rewrite inc_in_flight_to_backup_nil. omega.
   Qed.
 
   Theorem primary_ge_backup :
@@ -273,5 +273,176 @@ Section Counter.
     intros.
     apply backup_plus_network_eq_primary in H.
     auto with *.
+  Qed.
+
+  Definition trace_inputs (tr : list (name * (input + list output))) : nat :=
+    length (filterMap (fun e => match e with
+                             | (primary, inl i) => Some i
+                             | _ => None
+                             end) tr).
+  Lemma trace_inputs_app :
+    forall tr1 tr2,
+      trace_inputs (tr1 ++ tr2) = trace_inputs tr1 + trace_inputs tr2.
+  Proof.
+    unfold trace_inputs.
+    intros.
+    rewrite filterMap_app.
+    rewrite app_length. auto.
+  Qed.
+
+  Definition trace_outputs (tr : list (name * (input + list output))) : nat :=
+    length (filterMap (fun e => match e with
+                             | (primary, inr [o]) => Some o
+                             | _ => None
+                             end) tr).
+
+  Lemma trace_outputs_app :
+    forall tr1 tr2,
+      trace_outputs (tr1 ++ tr2) = trace_outputs tr1 + trace_outputs tr2.
+  Proof.
+    unfold trace_outputs.
+    intros.
+    rewrite filterMap_app.
+    rewrite app_length. auto.
+  Qed.
+
+  Definition ack_in_flight_to_primary (l : list packet) : nat :=
+    length (filterMap
+              (fun p => if msg_eq_dec (pBody p) ack
+                     then if name_eq_dec (pDst p) primary
+                          then Some tt else None
+                     else None)
+              l).
+
+  Lemma ack_in_flight_to_primary_app :
+    forall xs ys,
+      ack_in_flight_to_primary (xs ++ ys) = ack_in_flight_to_primary xs + ack_in_flight_to_primary ys.
+  Proof.
+    unfold ack_in_flight_to_primary.
+    intros.
+    rewrite filterMap_app.
+    rewrite app_length. auto.
+  Qed.
+
+  Lemma ack_in_flight_to_primary_backup :
+    forall p,
+      pDst p = backup ->
+      ack_in_flight_to_primary [p] = 0.
+  Proof.
+    intros.
+    unfold ack_in_flight_to_primary.
+    simpl.
+    repeat break_match; try congruence; auto.
+  Qed.
+
+
+  Lemma InputHandler_trace_preserved :
+    forall h i d u o d' l,
+      InputHandler h i d = (u, o, d', l) ->
+      trace_inputs [(h, inl i)] =
+      trace_outputs [(h, inr o)] +
+      inc_in_flight_to_backup (send_packets h l) +
+      ack_in_flight_to_primary (send_packets h l).
+  Proof.
+    unfold InputHandler, PrimaryInputHandler, BackupInputHandler.
+    simpl.
+    intros.
+    monad_unfold.
+    repeat break_match; find_inversion; compute; auto.
+  Qed.
+
+  Lemma NetHandler_trace_preserved :
+    forall p d u o d' l,
+      NetHandler (pDst p) (pBody p) d = (u, o, d', l) ->
+      inc_in_flight_to_backup [p] +
+      ack_in_flight_to_primary [p] =
+      trace_outputs [((pDst p), inr o)] +
+      inc_in_flight_to_backup (send_packets (pDst p) l) +
+      ack_in_flight_to_primary (send_packets (pDst p) l).
+  Proof.
+    unfold NetHandler, PrimaryNetHandler, BackupNetHandler.
+    intros.
+    monad_unfold.
+    destruct p. simpl in *.
+    repeat break_match; find_inversion; simpl; try rewrite inc_in_flight_to_backup_nil;
+    unfold Data in *; compute;
+    auto with *.
+  Qed.
+
+  Lemma trace_inputs_output :
+    forall h os,
+      trace_inputs [(h, inr os)] = 0.
+  Proof.
+    intros.
+    unfold trace_inputs.
+    simpl. repeat break_match; simpl; congruence.
+  Qed.
+
+  Lemma trace_outputs_input :
+    forall h i,
+      trace_outputs [(h, inl i)] = 0.
+  Proof.
+    intros.
+    unfold trace_outputs.
+    simpl. repeat break_match; simpl; congruence.
+  Qed.
+
+  Lemma trace_outputs_backup :
+    forall e,
+      trace_outputs [(backup, e)] = 0.
+  Proof.
+    auto.
+  Qed.
+
+  Lemma inputs_eq_outputs_plus_inc_plus_ack :
+    forall net tr,
+      step_m_star (params := Counter_MultiParams) step_m_init net tr ->
+      trace_inputs tr = trace_outputs tr +
+                        inc_in_flight_to_backup (nwPackets net) +
+                        ack_in_flight_to_primary (nwPackets net).
+  Proof.
+    intros.
+    remember step_m_init as y in *.
+    revert Heqy.
+    induction H using refl_trans_1n_trace_n1_ind; intros; subst.
+    - reflexivity.
+    - concludes.
+      match goal with
+      | [ H : step_m _ _ _ |- _ ] => invc H
+      end; simpl.
+      + find_apply_lem_hyp net_handlers_NetHandler.
+        repeat find_rewrite.
+        rewrite trace_inputs_app.
+        rewrite trace_outputs_app.
+        rewrite cons_is_app with (x := p) in *.
+        repeat rewrite inc_in_flight_to_backup_app in *.
+        repeat rewrite ack_in_flight_to_primary_app in *.
+        find_apply_lem_hyp NetHandler_trace_preserved.
+        destruct (pDst p) eqn:?.
+        * erewrite inc_in_flight_to_backup_cons_primary_dst in * by eauto.
+          rewrite trace_inputs_output in *. simpl in  *. omega.
+        * rewrite ack_in_flight_to_primary_backup in * by auto.
+          rewrite trace_outputs_backup in *. unfold send_packets in *.
+          simpl in *. rewrite <- plus_n_O in *. omega.
+      + find_apply_lem_hyp input_handlers_InputHandlers.
+        find_apply_lem_hyp InputHandler_trace_preserved.
+        rewrite cons_is_app.
+        repeat rewrite trace_inputs_app.
+        repeat rewrite trace_outputs_app.
+        repeat rewrite inc_in_flight_to_backup_app in *.
+        repeat rewrite ack_in_flight_to_primary_app in *.
+        rewrite trace_outputs_input.
+        rewrite trace_inputs_output.
+        unfold send_packets in *. simpl in *. omega.
+  Qed.
+
+  Theorem inputs_ge_outputs :
+    forall net tr,
+      step_m_star (params := Counter_MultiParams) step_m_init net tr ->
+      trace_outputs tr <= trace_inputs tr.
+  Proof.
+    intros.
+    apply inputs_eq_outputs_plus_inc_plus_ack in H.
+    omega.
   Qed.
 End Counter.
